vale/code/arch/x64/interop/Vale.Wrapper.X64.Cpuid.fst
@@ -41,3 +41,11 @@ let check_avx512 () =
 let check_osxsave () =
   let (x, _) = Vale.Stdcalls.X64.Cpuid.check_osxsave () in //This is a call to the interop wrapper
   x
+
+let check_avx_xcr0 () =
+  let (x, _) = Vale.Stdcalls.X64.Cpuid.check_avx_xcr0 () in //This is a call to the interop wrapper
+  x
+
+let check_avx512_xcr0 () =
+  let (x, _) = Vale.Stdcalls.X64.Cpuid.check_avx512_xcr0 () in //This is a call to the interop wrapper
+  x
